deps/poulet4/lib/P4automata/Bisimulations/WPLeapsProofs.v
@@ -14,6 +14,8 @@ Require Import Poulet4.P4automata.Bisimulations.AlgorithmicLeaps.
 Require Import Poulet4.P4automata.Bisimulations.AlgorithmicLeapsProofs.
 Require Import Poulet4.P4automata.Bisimulations.WPLeaps.
 Require Import Poulet4.P4automata.Reachability.
+Require Import Poulet4.P4automata.Syntax.
+Require Import Poulet4.Utils.
 
 Section WPLeapsProofs.
 
@@ -50,47 +52,6 @@ Section WPLeapsProofs.
   Notation "R ⊨ S" := (interp_entailment a top {| e_prem := R; e_concl := S |}) (at level 40).
   Notation δ := step.
 
-  Lemma interp_crel_app:
-    forall R1 R2 q1 q2,
-      interp_crel a top (R1 ++ R2) q1 q2 <->
-      interp_crel a top R1 q1 q2 /\
-      interp_crel a top R2 q1 q2.
-  Proof.
-    intros.
-    induction R1; cbn; intuition.
-    induction R2; intuition.
-  Qed.
-
-  Lemma pre_bisimulation_implies_interp_crel:
-    forall R T q1 q2,
-      pre_bisimulation a (WP.wp r) top R T q1 q2 ->
-      top q1 q2 ->
-      interp_crel a top (T ++ R) q1 q2.
-  Proof.
-    intros.
-    induction H0.
-    - rewrite app_nil_l.
-      apply H0; simpl; auto.
-    - destruct H0; [|contradiction].
-      specialize (IHpre_bisimulation H1).
-      repeat rewrite interp_crel_app in *.
-      rewrite interp_crel_cons in *.
-      intuition.
-    - destruct H0; [contradiction|].
-      specialize (IHpre_bisimulation H1).
-      repeat rewrite interp_crel_app in *.
-      rewrite interp_crel_cons in *.
-      intuition.
-  Qed.
-
-  Lemma interp_rels_vs_interp_crel:
-    forall q1 q2 R,
-      interp_rels top (map (interp_conf_rel a) R) q1 q2 <->
-      interp_crel a top R q1 q2.
-  Proof.
-    induction R; intuition.
-  Qed.
-
   Lemma pre_bisimulation_embed:
     forall R T q1 q2,
       pre_bisimulation a (WP.wp r) top R T q1 q2 ->
@@ -103,12 +64,10 @@ Section WPLeapsProofs.
   Proof.
     intros.
     induction H0.
-    - apply AlgorithmicLeaps.PreBisimulationClose.
-      now rewrite interp_rels_vs_interp_crel.
+    - now apply AlgorithmicLeaps.PreBisimulationClose.
     - apply AlgorithmicLeaps.PreBisimulationSkip.
       + intros.
         destruct H0; [|contradiction].
-        rewrite interp_rels_vs_interp_crel in H3.
         now apply i.
       + apply IHpre_bisimulation.
     - eapply AlgorithmicLeaps.PreBisimulationExtend.
@@ -116,432 +75,67 @@ Section WPLeapsProofs.
         destruct H0; [contradiction|].
         apply n.
         unfold interp_entailment; simpl; intros.
-        apply H4.
-        now rewrite interp_rels_vs_interp_crel.
+        now apply H4.
       + fold (map (interp_conf_rel a) T).
         rewrite map_cons, map_app in IHpre_bisimulation.
         exact IHpre_bisimulation.
       + intros.
-        rewrite interp_rels_vs_interp_crel in H4.
         eapply wp_safe; auto.
         rewrite <- H2.
         exact H4.
   Admitted.
 
-  Lemma interp_rels_intersect_top:
-    forall q1 q2 R,
-      interp_rels top R q1 q2 <->
-      (top ⊓ interp_rels top R) q1 q2.
+  Lemma not_equally_accepting_correct q1 q2:
+    not_equally_accepting S1 S2 H a (conf_to_state_template q1,
+                                     conf_to_state_template q2) = false ->
+    accepting q1 <-> accepting q2.
   Proof.
-    induction R; cbn; intuition.
+    unfold not_equally_accepting, accepting; simpl; intros.
+    destruct (conf_state q1), (conf_state q2);
+    try destruct b; try destruct b0;
+    split; intros; congruence.
   Qed.
 
-  Opaque top.
-
-  Lemma interp_crel_quantify:
-    forall R (q1 q2: conf),
-      ⟦R⟧ q1 q2 <->
-      top q1 q2 /\ (forall phi, In phi R -> ⦇phi⦈ q1 q2).
-  Proof.
-    intros; induction R.
-    - intuition.
-    - rewrite interp_crel_cons, IHR; intuition.
-      destruct H4; subst; intuition.
-  Qed.
-
-  Transparent top.
-
-  Lemma interp_crel_nodup:
-    forall R (q1 q2: conf),
-      ⟦R⟧ q1 q2 <->
-      ⟦nodup (conf_rel_eq_dec (a := a)) R⟧ q1 q2.
-  Proof.
-    intros.
-    repeat rewrite interp_crel_quantify.
-    now setoid_rewrite nodup_In.
-  Qed.
-
-  Lemma init_vs_accepting:
+  Lemma mk_init_accepting:
     forall (q1 q2: conf),
       ⟦mk_init _ _ _ _ (length (valid_state_pairs a)) s1 s2⟧ q1 q2 ->
       (accepting q1 <-> accepting q2).
   Proof.
     intros.
-    unfold mk_init in H0.
-    rewrite <- interp_crel_nodup in H0.
-    unfold mk_partition in H0.
-    rewrite interp_crel_quantify in H0.
-    destruct H0.
-    unfold top in H0.
-    unfold r in H0.
-    unfold accepting.
-    split; intros.
-    assert (~ not_equally_accepting S1 S2 H a (conf_to_state_template q1, conf_to_state_template q2) = true).
-    intro.
-    assert (⦇ mk_rel S1 S2 H a (conf_to_state_template q1, conf_to_state_template q2) ⦈ q1 q2).
-    apply H1.
-    apply in_map.
-    rewrite filter_In.
-    split; auto.
-    unfold mk_rel in H4.
-    unfold interp_conf_rel in H4.
-    vm_compute in H4.
-    apply H4.
-    intuition.
-    exact tt.
-    rewrite Bool.not_true_iff_false in H3.
-    unfold not_equally_accepting in H3.
-    unfold conf_to_state_template in H3.
-    simpl in H3.
-    rewrite H2 in H3.
-    destruct (conf_state q2).
-    discriminate.
-    destruct b.
-    reflexivity.
-    discriminate.
-    assert (~ not_equally_accepting S1 S2 H a (conf_to_state_template q1, conf_to_state_template q2) = true).
-    intro.
-    assert (⦇ mk_rel S1 S2 H a (conf_to_state_template q1, conf_to_state_template q2) ⦈ q1 q2).
-    apply H1.
-    apply in_map.
-    rewrite filter_In.
-    split; auto.
-    unfold mk_rel in H4.
-    unfold interp_conf_rel in H4.
-    vm_compute in H4.
-    apply H4.
-    intuition.
-    exact tt.
-    rewrite Bool.not_true_iff_false in H3.
-    unfold not_equally_accepting in H3.
-    unfold conf_to_state_template in H3.
-    simpl in H3.
-    rewrite H2 in H3.
-    destruct (conf_state q1).
-    discriminate.
-    destruct b.
-    reflexivity.
-    discriminate.
-  Qed.
-
-  Lemma reachable_states_closed r (p1 p2: Reachability.state_pair a):
-    (forall p, List.In p r -> valid_state_pair p) ->
-    List.In p1 (reachable_states' (length (valid_state_pairs a)) r) ->
-    List.In p2 (reachable_step [p1]) ->
-    List.In p2 (reachable_states' (length (valid_state_pairs a)) r).
-  Proof.
-    intros.
-    apply reachable_states_bound with (fuel := Datatypes.S (length (valid_state_pairs a))); auto.
-    unfold reachable_states'.
-    fold (reachable_states' (length (valid_state_pairs a)) r).
-    revert H2; apply reachable_step_mono.
-    unfold incl; intros.
-    destruct H2; try contradiction; now subst.
-  Qed.
-
-  Lemma follow_false q bs:
-    conf_state q = inr false ->
-    conf_state (follow (a := P4A.interp a) q bs) = inr false.
-  Proof.
-    revert q; induction bs; intros.
-    - now autorewrite with follow.
-    - autorewrite with follow.
-      apply IHbs.
-      unfold step.
-      destruct (Compare_dec.le_lt_dec _ _).
-      + simpl.
-        match goal with
-        | |- context [ (WP.P4A.P4A.update' _ _ ?t _) ] =>
-          generalize t
-        end.
-        intros.
-        destruct (WP.P4A.P4A.conf_state q).
-        * discriminate.
-        * autorewrite with update'.
-          autorewrite with transitions'.
-          reflexivity.
-      + simpl.
-        apply H0.
-  Qed.
-
-  Lemma buf_len_halted q b:
-    conf_state q = inr b ->
-    conf_buf_len (a := P4A.interp a) q = 0.
-  Proof.
-    intros.
-    destruct q.
-    simpl in *.
-    rewrite H0 in conf_buf_sane.
-    autorewrite with size' in conf_buf_sane.
-    Lia.lia.
-  Qed.
-
-  Lemma foo q1 bs:
-    1 <= length bs <= configuration_room_left q1 ->
-    In (conf_to_state_template (follow q1 bs))
-      (advance (a := a)
-         (length bs)
-         (conf_to_state_template q1) (st_state (conf_to_state_template q1))).
-  Proof.
-    intros.
-    unfold advance.
-    unfold conf_to_state_template at 2; simpl.
-    destruct (conf_state q1) eqn:?.
-    - unfold configuration_room_left in H0.
-      rewrite Heqs in H0.
-      autorewrite with size' in H0.
-      destruct (Compare_dec.le_gt_dec _ _).
-      + simpl in H0.
-        assert (P4A.size (S := Reachability.S S1 S2) a s = conf_buf_len q1 + length bs) by Lia.lia.
-        clear l.
-        destruct H0.
-        clear H2.
-        revert q1 Heqs H1.
-        induction bs; intros.
-        * simpl in H1.
-          pose proof (conf_buf_sane q1).
-          rewrite Heqs in H2.
-          autorewrite with size' in H2.
-          simpl in H2.
-          Lia.lia.
-        * destruct bs.
-          -- autorewrite with follow.
-             simpl in H1.
-             unfold step.
-             destruct (Compare_dec.le_lt_dec _ _).
-             ++ simpl.
-                match goal with
-                | |- context [ WP.P4A.P4A.update' _ _ ?t _ ] =>
-                  generalize t
-                end; intros.
-                unfold conf_to_state_template.
-                simpl.
-                apply in_map_iff.
-                eexists.
-                split.
-                reflexivity.
-                destruct (WP.P4A.P4A.conf_state q1); [|discriminate].
-                autorewrite with update'.
-                autorewrite with transitions'.
-                unfold possible_next_states.
-                unfold WP.P4A.P4A.transitions.
-                simpl.
-                unfold P4A.transitions.
-                unfold P4A.eval_trans.
-                inversion Heqs.
-                subst.
-                destruct (P4A.st_trans _).
-                apply in_eq.
-                induction cases.
-                simpl.
-                left; reflexivity.
-                simpl P4A.eval_sel.
-                destruct (P4A.match_pat _ _ _ _).
-                rewrite map_cons.
-                apply in_cons.
-                apply in_eq.
-                rewrite map_cons.
-                destruct IHcases.
-                rewrite H2 at 2.
-                apply in_eq.
-                apply in_cons.
-                apply in_cons.
-                apply H2.
-             ++ exfalso.
-                rewrite Heqs in l.
-                autorewrite with size' in l.
-                simpl in l.
-                Lia.lia.
-          -- rewrite follow_equation_2.
-             apply IHbs.
-             ++ simpl.
-                Lia.lia.
-             ++ unfold step.
-                destruct (Compare_dec.le_lt_dec _ _).
-                ** exfalso.
-                   rewrite Heqs in l.
-                   autorewrite with size' in l.
-                   simpl in l.
-                   simpl in H1.
-                   Lia.lia.
-                ** now simpl.
-             ++ unfold step.
-                destruct (Compare_dec.le_lt_dec _ _).
-                ** exfalso.
-                   rewrite Heqs in l.
-                   autorewrite with size' in l.
-                   simpl in l.
-                   simpl in H1.
-                   Lia.lia.
-                ** simpl in *.
-                   Lia.lia.
-      + clear H0; revert q1 s Heqs g; induction bs; intros.
-        * autorewrite with follow.
-          left.
-          unfold conf_to_state_template.
-          now f_equal.
-        * autorewrite with follow.
-          replace (conf_buf_len q1 + length (a0 :: bs))
-          with ((1 + conf_buf_len q1) + length bs) by (simpl; Lia.lia).
-          replace (1 + conf_buf_len q1) with (conf_buf_len (δ q1 a0)).
-          apply IHbs.
-          -- unfold step.
-             destruct (Compare_dec.le_lt_dec _ _).
-             ++ exfalso.
-                rewrite Heqs in l.
-                autorewrite with size' in l.
-                simpl in l, g.
-                Lia.lia.
-             ++ now simpl.
-          -- unfold step.
-             destruct (Compare_dec.le_lt_dec _ _).
-             ++ exfalso.
-                rewrite Heqs in l.
-                autorewrite with size' in l.
-                simpl in l, g.
-                Lia.lia.
-             ++ simpl in *.
-                Lia.lia.
-          -- unfold step.
-             destruct (Compare_dec.le_lt_dec _ _).
-             ++ exfalso.
-                rewrite Heqs in l.
-                autorewrite with size' in l.
-                simpl in l, g.
-                Lia.lia.
-             ++ now simpl.
-    - destruct bs.
-      + simpl in H0; Lia.lia.
-      + autorewrite with follow.
-        destruct q1.
-        simpl in Heqs.
-        unfold step.
-        simpl.
-        destruct (Compare_dec.le_lt_dec _ _).
-        destruct (conf_state).
-        discriminate.
-        inversion Heqs.
-        autorewrite with transitions'.
-        left.
-        unfold conf_to_state_template.
-        f_equal.
-        rewrite follow_false.
-        reflexivity.
-        simpl.
-        reflexivity.
-        rewrite buf_len_halted with (b := false).
-        reflexivity.
-        apply follow_false.
-        simpl.
-        reflexivity.
-        right.
-        rewrite Heqs in l.
-        autorewrite with size' in l.
-        Lia.lia.
+    apply not_equally_accepting_correct, Bool.not_true_iff_false; intro.
+    apply interp_crel_nodup, interp_crel_quantify in H0; destruct H0.
+    specialize (H2 (mk_rel _ _ _ _ (conf_to_state_template q1,
+                                    conf_to_state_template q2))).
+    modus_ponens H2; [ apply in_map, filter_In; intuition |].
+    unfold interp_conf_rel in H2; simpl interp_store_rel in H2.
+    modus_ponens H2; [ vm_compute; intuition |].
+    simpl bval in H2; now specialize (H2 tt).
   Qed.
 
   Lemma top_closed q1 q2 bs:
-    length bs = reads_left (conf_to_state_template q1, conf_to_state_template q2) ->
+    length bs = reads_left (conf_to_state_template q1,
+                            conf_to_state_template q2) ->
     top q1 q2 ->
     top (follow q1 bs) (follow q2 bs).
   Proof.
     unfold top, r, reachable_states; intros.
     eapply reachable_states_closed.
-    - intros.
-      destruct H2; try contradiction.
-      subst.
+    - intros; destruct H2; try contradiction; subst.
       unfold valid_state_pair, valid_state_template; simpl.
       split; apply Syntax.t_has_extract.
     - exact H1.
     - unfold reachable_step.
-      apply nodup_In.
-      simpl.
+      apply nodup_In; simpl.
       rewrite app_nil_r, in_app_iff; left.
-      unfold reachable_pair_step.
-      unfold reachable_pair_step'.
-      apply in_prod.
-      + rewrite <- H0.
-        simpl.
-        destruct (conf_state q1) eqn:?.
-        * rewrite <- Heqs.
-          apply foo.
-          split.
-          -- rewrite H0.
-             unfold reads_left; simpl.
-             pose proof (conf_buf_sane q1).
-             pose proof (conf_buf_sane q2).
-             destruct (conf_state q1), (conf_state q2);
-             autorewrite with size' in H2, H3;
-             simpl in H2, H3;
-             Lia.lia.
-          -- unfold reads_left in H0; simpl in H0.
-             unfold configuration_room_left.
-             pose proof (conf_buf_sane q1).
-             rewrite Heqs in *.
-             autorewrite with size' in *;
-             simpl in H2; simpl;
-             destruct (conf_state q2);
-             try Lia.lia.
-        * destruct bs.
-          -- unfold reads_left in H0.
-             simpl in H0.
-             pose proof (conf_buf_sane q1).
-             pose proof (conf_buf_sane q2).
-             destruct (conf_state q1), (conf_state q2);
-             autorewrite with size' in *;
-             simpl in H2, H3;
-             Lia.lia.
-          -- autorewrite with follow.
-             eapply LeapsProofs.step_done in Heqs.
-             unfold conf_to_state_template.
-             rewrite follow_false.
-             erewrite buf_len_halted.
-             simpl.
-             left; reflexivity.
-             apply follow_false.
-             exact Heqs.
-             exact Heqs.
-      + rewrite <- H0.
-        simpl.
-        destruct (conf_state q2) eqn:?.
-        * rewrite <- Heqs.
-          apply foo.
-          split.
-          -- rewrite H0.
-             unfold reads_left; simpl.
-             pose proof (conf_buf_sane q1).
-             pose proof (conf_buf_sane q2).
-             destruct (conf_state q1), (conf_state q2);
-             autorewrite with size' in H2, H3;
-             simpl in H2, H3;
-             Lia.lia.
-          -- unfold reads_left in H0; simpl in H0.
-             unfold configuration_room_left.
-             pose proof (conf_buf_sane q2).
-             rewrite Heqs in *.
-             autorewrite with size' in *;
-             simpl in H2; simpl;
-             destruct (conf_state q1);
-             try Lia.lia.
-        * destruct bs.
-          -- unfold reads_left in H0.
-             simpl in H0.
-             pose proof (conf_buf_sane q1).
-             pose proof (conf_buf_sane q2).
-             destruct (conf_state q1), (conf_state q2);
-             autorewrite with size' in *;
-             simpl in H2, H3;
-             Lia.lia.
-          -- autorewrite with follow.
-             eapply LeapsProofs.step_done in Heqs.
-             unfold conf_to_state_template.
-             rewrite follow_false.
-             erewrite buf_len_halted.
-             simpl.
-             left; reflexivity.
-             apply follow_false.
-             exact Heqs.
-             exact Heqs.
+      unfold reachable_pair_step, reachable_pair_step'.
+      apply in_prod; rewrite <- H0; simpl.
+      + eapply advance_correct; try typeclasses eauto; rewrite H0.
+        * intros; apply reads_left_upper_bound with (s := s); auto.
+        * apply reads_left_lower_bound.
+      + eapply advance_correct; try typeclasses eauto; rewrite H0;
+        setoid_rewrite reads_left_commutative.
+        * intros; apply reads_left_upper_bound with (s := s); auto.
+        * apply reads_left_lower_bound.
   Qed.
 
   Lemma wp_leaps_implies_bisim_leaps:
@@ -556,9 +150,9 @@ Section WPLeapsProofs.
     with (R := []) (T := map (interp_conf_rel a) init) (top := top).
     - simpl interp_rels at 1.
       unfold coaccepting; intros.
-      erewrite init_vs_accepting.
+      erewrite mk_init_accepting.
       + reflexivity.
-      + rewrite <- interp_rels_vs_interp_crel, interp_rels_intersect_top.
+      + unfold interp_crel; rewrite interp_rels_intersect_top.
         exact H2.
     - simpl interp_rels at 1.
       unfold follow_closed; intros.
